pointSubAssign impl -> low

src/zksync_verifier.ec
@@ -520,3 +520,48 @@ proof.
   inline*. wp. skip. progress.
   inline*. wp. skip. progress.
 qed.
+
+module PointSubAssign = {
+  proc low(usr_p1, usr_p2) =
+  {
+    var _1, _5, _6, _9, _15, _16, tmp71;
+    _1 <@ Primops.mload(usr_p1);
+    Primops.mstore(W256.zero, _1);
+    _5 <@ Primops.mload(usr_p1 + W256.of_int 32);
+    Primops.mstore(W256.of_int 32, _5);
+    _6 <@ Primops.mload(usr_p2);
+    Primops.mstore(W256.of_int 64, _6);
+    _9  <@ Primops.mload(usr_p2 + W256.of_int 32);
+    Primops.mstore(W256.of_int 96, W256.of_int 21888242871839275222246405745257275088696311157297823662689037894645226208583 - _9);
+    _15 <@ Primops.gas();
+    _16 <@ Primops.staticcall(_15, W256.of_int 6, W256.zero, W256.of_int 128, usr_p1, W256.of_int 64);
+    if ((bool_of_uint256 (PurePrimops.iszero _16)))
+      {
+      tmp71 <@ Verifier_1261.usr_revertWithMessage(W256.of_int 28, (W256.of_int STRING));
+      }
+  }
+}.
+
+lemma usr_pointSubAssign_actual_matches_low (x y : uint256) : equiv [
+    Verifier_1261.usr_pointSubAssign ~ PointSubAssign.low :
+      ={Primops.memory} /\
+      ={arg} /\
+      ={Primops.reverted} /\
+      !Primops.reverted{1}
+      ==>
+        (Primops.reverted{1} <=> Primops.reverted{2}) /\
+        (!Primops.reverted{1}) =>
+        forall (idx: uint256),
+        Primops.memory{1}.[idx] =
+        Primops.memory{2}.[idx]
+      ].
+proof.
+  proc.
+  seq 16 7: (#pre /\ ={_1} /\ _2{1} = W256.zero /\ _3{1} = W256.of_int 32 /\ _4{1} = usr_p1{1} + _3{1}
+            /\ ={_5, _6, _9} /\ _7{1} = W256.of_int 64 /\ _8{1} = usr_p2{1} + _3{1}).
+  inline*. wp. skip. progress. sp.
+  seq 7 3: (#pre /\ _13{1} = W256.of_int 128 /\ _14{1} = W256.of_int 6 /\ ={_15, _16}).
+  inline*. wp. skip. progress.
+  inline*. wp. skip. progress.
+qed.  
+  
